BignumTest/ArmRev/ShiftType.lean
@@ -4,44 +4,21 @@ open Bignum.ArmRev
 
 -- LSL
 
-/-- info: 0x00000008#32 -/
-#guard_msgs in
-#eval ShiftType.LSL.shift 1 0x4#32
-
-/-- info: 0x00000000#32 -/
-#guard_msgs in
-#eval ShiftType.LSL.shift 1 0x80000000#32
+example : ShiftType.LSL.shift 1 4#32 = 8#32 := by rfl
+example : ShiftType.LSL.shift 1 0x80000000#32 = 0#32 := by rfl
 
 -- LSR
 
-/-- info: 0x00000002#32 -/
-#guard_msgs in
-#eval ShiftType.LSR.shift 1 0x4#32
-
-/-- info: 0x00000000#32 -/
-#guard_msgs in
-#eval ShiftType.LSR.shift 1 0x1#32
+example : ShiftType.LSR.shift 1 4#32 = 2#32 := by rfl
+example : ShiftType.LSR.shift 1 1#32 = 0#32 := by rfl
 
 -- ASR
 
-/-- info: 0x00000000#32 -/
-#guard_msgs in
-#eval ShiftType.ASR.shift 1 0x0#32
-
-/-- info: 0x00000000#32 -/
-#guard_msgs in
-#eval ShiftType.ASR.shift 1 0x1#32
-
-/-- info: 0x2#4 -/
-#guard_msgs in
-#eval ShiftType.ASR.shift 1 0x5#4
+example : ShiftType.ASR.shift 1 0#32 = 0#32 := by rfl
+example : ShiftType.ASR.shift 1 1#32 = 0#32 := by rfl
+example : ShiftType.ASR.shift 1 5#4 = 2#4 := by rfl
 
 -- ROR
 
-/-- info: 0x80#8 -/
-#guard_msgs in
-#eval ShiftType.ROR.shift 1 0x1#8
-
-/-- info: 0x1#4 -/
-#guard_msgs in
-#eval ShiftType.ROR.shift 1 0x2#4
+example : ShiftType.ROR.shift 1 1#8 = 0x80#8 := by rfl
+example : ShiftType.ROR.shift 1 2#4 = 1#4 := by rfl
